Mark

theories/lambdaSolve.v
@@ -2,7 +2,15 @@ Require Import String.
 Require Import qterm.
 Require Import lambdaFacts.
 
+(*
+The goal of these tactics is to reduce terms to a normal form.
+In order for them to work, we need to assume that the input terms have a particular form:
+All QTerms should consist of lam, app, var, pair, pi1, pi2, const, and coq variables.
+Any lifts should be around a coq variable.
 
+There should not be any lifts anywhere else or subst forms anywhere at all
+except during intermediate states.
+*)
 
 Ltac compute_subst := repeat (try rewrite subst_app ;
                           try (rewrite subst_lam ; simpl) ;
@@ -40,13 +48,94 @@ Ltac lambda_solve :=
     (*)*)
 .
 
+Theorem test_lambda_solve_0
+        (t : QTerm)
+  : <fun x => `t> = <fun y => `t>.
+Proof.
+  repeat lambda_solve.
+Abort. (* This shouldn't be true, because t could have x or y in it. *)
+
+(* We need to hide Mark in a module *)
+Module Type HowToHideMark.
+  Parameter Mark : forall {X : Type}, X -> X. (* He hides in here where no one can see him *)
+  Parameter MarkIsJustId : forall {X : Type} {x : X}, Mark x = x.
+End HowToHideMark.
+Module HiddenMark : HowToHideMark.
+  Definition Mark {X : Type} (x : X) := x.
+  Theorem MarkIsJustId {X : Type} {x : X} : Mark x = x.
+  Proof.
+    intros.
+    reflexivity.
+  Qed.
+End HiddenMark.
+
+Import HiddenMark.
+
+Theorem mark_stuck : forall t s1 i1 s2 i2 t',
+    subst s1 i1 t' (lift s2 i2 t) = subst s1 i1 t' ((Mark lift) s2 i2 t).
+Proof.
+  rewrite MarkIsJustId.
+  reflexivity.
+Qed.
+
+Theorem swap_marked_lift : forall (s1 s2 : string) (i1 i2 : nat) (t : QTerm),
+    (Mark lift) s1 i1 (lift s2 i2 t) =
+      lift s2 (if (s1 =? s2)%string then S i2 else i2) ((Mark lift) s1 i1 t).
+Proof.
+  rewrite MarkIsJustId.
+  apply lift_lift.
+Qed.
+
+Ltac fix_subst_lifts :=
+  repeat (
+      (* First, cancel any substs and lifts that already match*)
+      repeat rewrite subst_lift;
+      (* Next, mark any lifts under a subst as being the wrong one *)
+      repeat rewrite mark_stuck;
+      (* Next, push the marked lift down *)
+      repeat (rewrite swap_marked_lift ; simpl)
+    );
+  (* When we are done, remove Mark *)
+  repeat rewrite MarkIsJustId.
+
+
+Theorem test_lambda_solve_1
+        (t : QTerm)
+  : <fun x => `t [x]> = <fun y => `t [y]>.
+Proof.
+  repeat lambda_solve.
+  (* In order to be able to cancel out lifts and substitutions in general, I will need
+   simultaneous lifts and substitutions. There is not a solution where we commute the subs
+   and lifts past each other, because that isn't always possible.
+   If I make the assumption that we only have lifts around metavariables, and that metavariables
+   are always in the empty context, then I think I can get away with only having simultaneous
+   lifts but not substitutions. *)
+  (*
+    One possible solution: write a tactic which repeatedly raised lift x through other lifts,
+    and a tactic which searches for a subst around a lift and returns the x from the subst
+    so that it can know which thing to looks for.
+    A problem is how this would work with multiple lifts of the same name but different
+    debruin indices.
+    Note that you can just match on expressions however you want in LTac:
+    https://softwarefoundations.cis.upenn.edu/plf-current/LibTactics.html
+   *)
+  fix_subst_lifts.
+  Check subst_lift.
+  Check alpha.
+  rewrite lift_lift. simpl.
+  rewrite subst_lift.
+  reflexivity.
+Qed.
+  
+
 Theorem test_lambda_solve
         (t1 t2 : QTerm)
-        (H1 : <Pi , A , fun x => `t1 [x]> = <Pi , A , fun x => `t2 [x]>)
+        (H1 : <fun x => `t1 [x]> = <fun x => `t2 [x]>)
   : <fun x => `t1[x]> = <fun y => `t2[x]>.
 Proof.
   repeat lambda_solve.
   rewrite H0.
+  Check subst_lift.
   rewrite subst_lift.
   (* Some axiom is wrong. *)
   
